Further work hashMaps

CertifyingDatalog/HashSets.lean
@@ -8,7 +8,179 @@ import Mathlib.Data.Bool.AllAny
 
 namespace Std
 section HashMap
-variable {A:Type} [Hashable A] [BEq A] [LawfulBEq A] [DecidableEq A] {B: Type} [DecidableEq B]
+variable {A:Type} [Hashable A] [DecidableEq A] {B: Type} [DecidableEq B]
+
+lemma Array.mem_if_exists (as: Array A) (a:A): a ∈ as ↔ ∃ (i: Fin as.size), a = as[i] :=
+by
+  cases as with
+  | mk l  =>
+    rw [Array.mem_def]
+    simp
+    rw [List.mem_iff_get]
+    constructor
+    intro h
+    rcases h with ⟨n, get_n⟩
+    use n
+    apply Eq.symm
+    apply get_n
+
+    intro h
+    rcases h with ⟨i, get_i⟩
+    use i
+    apply Eq.symm
+    apply get_i
+
+lemma List.mem_set (l: List A)(i: Fin l.length) (a d: A): a ∈ l.set i d ↔ a = d ∨ ∃ (j: Fin l.length), j ≠ i ∧ a = l[j] := by
+  simp
+  induction l with
+  | nil =>
+    exfalso
+    simp at i
+    have h: i.val < 0 := i.isLt
+    simp at h
+  | cons hd tl ih =>
+    cases hi: i.val with
+    | zero =>
+      simp
+      rw [List.mem_iff_get]
+      constructor
+      intro h
+      cases h with
+      | inl a_d =>
+        left
+        apply a_d
+      | inr get_a =>
+        rcases get_a with ⟨k, get_a⟩
+        right
+        have isLt_k: Nat.succ k.val < (hd::tl).length := by
+          simp
+          apply Nat.succ_lt_succ
+          apply k.isLt
+        use Fin.mk (Nat.succ k.val) isLt_k
+        constructor
+        cases i with
+        | mk i_val isLt_i =>
+          simp
+          simp at hi
+          rw [hi]
+          simp
+        rw [← get_a]
+        rw [← List.get_cons_succ (a:=hd)]
+
+      intro h
+      cases h with
+      | inl ad =>
+        left;apply ad
+      | inr h =>
+        rcases h with ⟨j, j_i, get_j⟩
+        right
+        cases hj:j.val with
+        | zero =>
+          rw [← Ne.def,←  Fin.val_ne_iff, hj, hi] at j_i
+          simp at j_i
+        | succ k =>
+          have isLt_k: k < tl.length := by
+            rw [← Nat.succ_lt_succ_iff, ← hj]
+            apply j.isLt
+          use Fin.mk k isLt_k
+          rw [get_j]
+          have hj': j = Fin.mk k.succ _ := by
+            rw [Fin.ext_iff]
+            simp
+            apply hj
+            rw [Nat.succ_lt_succ_iff]
+            apply isLt_k
+          rw [hj', List.get_cons_succ]
+    | succ m =>
+      rw [List.set_succ]
+      simp
+      have isLt_m: m < tl.length := by
+        rw [← Nat.succ_lt_succ_iff, ← hi]
+        apply i.isLt
+      specialize ih (Fin.mk m isLt_m)
+      rw [ih]
+      constructor
+      intro h
+      cases h with
+      | inl ahd =>
+        right
+        use 0
+        simp [ahd]
+        rw [← Ne.def, ← Fin.val_ne_iff]
+        simp [Fin.ext, hi]
+      | inr h =>
+        cases h with
+        | inl ad =>
+          left;apply ad
+        | inr h =>
+          rcases h with ⟨j,j_i, get_j⟩
+          right
+          have isLt_j: j.val.succ < (hd::tl).length := by
+            simp
+            rw [Nat.succ_lt_succ_iff]
+            apply j.isLt
+          use Fin.mk j.val.succ isLt_j
+          constructor
+          rw [← Ne.def, ← Fin.val_ne_iff]
+          simp
+          rw [hi]
+          rw [← Ne.def,Nat.succ_ne_succ]
+          rw [← Ne.def, ← Fin.val_ne_iff] at j_i
+          simp at j_i
+          rw [Ne.def]
+          apply j_i
+
+          simp
+          apply get_j
+
+
+      intro h
+      cases h with
+      | inl ad =>
+        right;left;apply ad
+      | inr h =>
+        rcases h with ⟨j, j_i, get_j⟩
+        cases hj: j.val with
+        | zero =>
+          left
+          rw [get_j]
+          have j_zero: j = 0 := by
+            rw [Fin.ext_iff]
+            apply hj
+          rw [j_zero, List.get_cons_zero]
+        | succ n =>
+          right
+          right
+          have isLt_n: n < tl.length := by
+            rw [← Nat.succ_lt_succ_iff, ← hj]
+            apply j.isLt
+          use Fin.mk n isLt_n
+          simp
+          constructor
+          rw [← Ne.def, ← Nat.succ_ne_succ, ← hj, ← hi]
+          rw [Fin.val_ne_iff]
+          apply j_i
+          have isLt_succ_n: n + 1 < (hd::tl).length := by
+            simp
+            rw [← Nat.succ_eq_add_one, Nat.succ_lt_succ_iff]
+            apply isLt_n
+          rw [get_j, ← List.get_cons_succ (a:=hd) (h:= isLt_succ_n)]
+          congr
+          rw [Fin.ext_iff]
+          simp [hj]
+
+
+
+
+lemma Array.mem_set (as: Array A) (i: Fin as.size) (a d: A): a ∈ as.set i d ↔ a = d ∨ ∃ (j: Fin as.size), j ≠ i ∧ a = as[j] :=
+by
+  cases as with
+  | mk data =>
+    unfold Array.set
+    rw [Array.mem_def]
+    simp
+    rw [List.mem_set]
+    tauto
 
 lemma Array.foldl_union (as: Array A) (f: A → Finset B) (S: Finset B) (b: B):  b ∈ (Array.foldl (fun x y => x ∪ f y) S as) ↔ b ∈ S ∨ ∃ (a: A), a ∈ as ∧ b ∈ f a :=
 by
@@ -24,6 +196,73 @@ by
       rw [ih]
       simp
       tauto
+
+lemma Array.foldl_union_set (as: Array A) (f: A → Finset B) (i: Fin as.size) (d: A) (S: Finset B) (b: B):  b ∈ (Array.foldl (fun x y => x ∪ f y) S (as.set i d)) ↔ b ∈ S ∨ b ∈ f d ∨  ∃ (j: Fin as.size), j ≠ i ∧ b ∈ f as[j] := by
+  rw [Array.foldl_union]
+  constructor
+  intro h
+  cases h with
+  | inl bS =>
+    left; apply bS
+  | inr a_set =>
+    rcases a_set with ⟨a, a_mem, b_a⟩
+    rw [Array.mem_def] at a_mem
+    unfold Array.set at a_mem
+    simp at a_mem
+    right
+    rw [List.mem_iff_get] at a_mem
+    rcases a_mem with ⟨n, get_n⟩
+    rw [List.get_set] at get_n
+    by_cases i_n: i.val = n.val
+    simp [i_n] at get_n
+    left
+    rw [get_n]
+    apply b_a
+
+    simp [i_n] at get_n
+    right
+    have isLt_n: n.val < as.size := by
+      unfold Array.size
+      have h: ↑n < List.length (List.set as.data (↑i) d) := by
+        apply n.2
+      admit
+    use Fin.mk n.val isLt_n
+    simp
+    constructor
+    rw [Fin.ext_iff]
+    simp [Eq.comm, i_n]
+
+    have as_n_a: as[n] = a := by
+      unfold_projs
+      unfold Array.get
+      apply get_n
+    simp at as_n_a
+    rw [as_n_a]
+    apply b_a
+
+  intro h
+  cases h with
+  | inl bS =>
+    left; apply bS
+  | inr get_a =>
+    right
+    cases get_a with
+    | inl bfd =>
+      use d
+      rw [Array.mem_def, Array.set]
+      simp
+      constructor
+      admit
+      apply bfd
+    | inr get_j =>
+      rcases get_j with ⟨j, j_i, b_j⟩
+      use as[j]
+      constructor
+      admit
+      apply b_j
+
+
+
 
 lemma Array.get_mem (as: Array A) (i: Fin as.size): as[i] ∈ as :=
 by
@@ -47,27 +286,6 @@ by
       simp
       rw [ih]
       tauto
-
-instance: DecidableEq (AssocList A B) :=
-  fun l1 l2 =>
-    match decEq l1.toList l2.toList with
-    | isTrue h => isTrue (Iff.mpr (AssocList.eq_iff_toList l1 l2) h)
-    | isFalse h => isFalse (Iff.mpr (Iff.ne (AssocList.eq_iff_toList l1 l2)) h)
-
-
-def HashMap.Imp.Buckets.keys' (buckets: HashMap.Imp.Buckets A B): Finset A := Array.foldl (fun x y => x ∪ (y.toList.map Prod.fst).toFinset) ∅ buckets.val
-
-
-
-lemma HashMap.Imp.Buckets.keys'_mem_iff (buckets: HashMap.Imp.Buckets A B) (a:A): a ∈ buckets.keys' ↔ ∃ (l: AssocList A B), l ∈ buckets.val ∧ l.contains a:=
-by
-  unfold keys'
-  rw [Array.foldl_union]
-  simp
-
-def HashMap.Imp.keys' (m: HashMap.Imp A B): Finset A :=
-  match m with
-  | ⟨_, buckets⟩ => buckets.keys'
 
 def AssocList.containsKeyValue (l: AssocList A B) (a: A) (b: B): Bool :=
   match l with
@@ -135,6 +353,88 @@ by
       simp [h]
 
 
+instance: DecidableEq (AssocList A B) :=
+  fun l1 l2 =>
+    match decEq l1.toList l2.toList with
+    | isTrue h => isTrue (Iff.mpr (AssocList.eq_iff_toList l1 l2) h)
+    | isFalse h => isFalse (Iff.mpr (Iff.ne (AssocList.eq_iff_toList l1 l2)) h)
+
+
+
+def HashMap.Imp.Buckets.kv (buckets: HashMap.Imp.Buckets A B): Finset (A × B) := Array.foldl (fun x y => x ∪ y.toList.toFinset) ∅ buckets.val
+
+def HashMap.Imp.kv (m: HashMap.Imp A B): Finset (A × B) := m.2.kv
+
+
+def HashMap.Imp.kv_member (m: HashMap.Imp A B) (a: A) (b:B): Bool :=
+  let ⟨_, buckets⟩ := m
+  let ⟨i, h⟩ := mkIdx buckets.2 (hash a |>.toUSize)
+  let bkt := buckets.1[i]
+
+  bkt.containsKeyValue a b
+
+lemma HashMap.Imp.kv_member_iff_in_kv (m: HashMap.Imp A B) (wf: HashMap.Imp.WF m) (a: A) (b:B): (a,b) ∈ m.kv ↔ HashMap.Imp.kv_member m a b = true :=
+by
+  cases m with
+  | mk size buckets =>
+    unfold Imp.kv
+    unfold Imp.Buckets.kv
+    rw [Array.foldl_union]
+    unfold kv_member
+    simp
+    rw [HashMap.Imp.WF_iff] at wf
+    simp at wf
+    constructor
+    intro h
+    rcases h with ⟨bkt, bkt_mem, ab_mem⟩
+    rw [Array.mem_if_exists] at bkt_mem
+    rcases bkt_mem with ⟨i, bkt_i⟩
+    have i_eq: i = (Fin.mk (mkIdx buckets.2 (hash a).toUSize).1.toNat (mkIdx buckets.2 (hash a).toUSize).2) := by
+      have hash_self: ∀ (i : Nat) (h : i < Array.size buckets.val), Std.AssocList.All (fun (k : A) (x : B) => USize.toNat (UInt64.toUSize (hash k) % Array.size buckets.val) = i) buckets.val[i] := by
+        rcases wf with ⟨_, wf⟩
+        apply wf.hash_self
+      specialize hash_self i i.isLt
+      unfold AssocList.All at hash_self
+      specialize hash_self (a,b)
+      rw [bkt_i] at ab_mem
+      specialize hash_self ab_mem
+      unfold mkIdx
+      simp
+      rw [Fin.ext_iff, ← hash_self]
+
+    rw [i_eq] at bkt_i
+    simp at bkt_i
+    rw [← bkt_i]
+    rw [← AssocList.mem_containsKeyValue_iff_mem_toList] at ab_mem
+    simp at ab_mem
+    apply ab_mem
+
+    intro h
+    use buckets.1.get (Fin.mk (mkIdx buckets.2 (hash a).toUSize).1.toNat (mkIdx buckets.2 (hash a).toUSize).2)
+    simp
+    constructor
+    exact Array.get_mem buckets.1 (Fin.mk (mkIdx buckets.2 (hash a).toUSize).1.toNat (mkIdx buckets.2 (hash a).toUSize).2)
+    rw [← AssocList.mem_containsKeyValue_iff_mem_toList]
+    exact h
+
+
+def HashMap.Imp.Buckets.keys' (buckets: HashMap.Imp.Buckets A B): Finset A := Array.foldl (fun x y => x ∪ (y.toList.map Prod.fst).toFinset) ∅ buckets.val
+
+
+
+lemma HashMap.Imp.Buckets.keys'_mem_iff (buckets: HashMap.Imp.Buckets A B) (a:A): a ∈ buckets.keys' ↔ ∃ (l: AssocList A B), l ∈ buckets.val ∧ l.contains a:=
+by
+  unfold keys'
+  rw [Array.foldl_union]
+  simp
+
+def HashMap.Imp.keys' (m: HashMap.Imp A B): Finset A :=
+  match m with
+  | ⟨_, buckets⟩ => buckets.keys'
+
+
+
+
 lemma HashMap.Imp.contains_iff (m: HashMap.Imp A B) (wf: HashMap.Imp.WF m): m.contains a ↔ a ∈ m.keys' :=
 by
   cases m with
@@ -194,6 +494,114 @@ by
     rw [← ab_a]
     apply ab_mem
 
+lemma HashMap.Imp.expand_go_mem (i : Nat) (source : Array (AssocList A B)) (target : Buckets A B) (bkt: AssocList A B): bkt ∈ (HashMap.Imp.expand.go i source target).1 ↔ bkt ∈ target.1 ∨ ∃ (j: Fin source.size), j.val ≥ i ∧ bkt = source[j] := by
+  induction' h:(source.size - i)  with n ih generalizing source i target
+
+  rw [Nat.sub_eq_zero_iff_le] at h
+  unfold expand.go
+  admit
+
+  unfold expand.go
+  have h_i: i < source.size := by
+    admit
+  simp [h_i]
+  specialize ih (i+1) (source.set (Fin.mk i h_i) AssocList.nil) (List.foldl (fun d x => reinsertAux d x.1 x.2) target (AssocList.toList source[i]))
+  simp at ih
+  have h': Array.size source - (i + 1) = n := by
+    admit
+  specialize ih h'
+  rw [ih]
+
+
+
+lemma HashMap.Imp.expand_preserves_mem  (size : Nat) (buckets : Buckets A B) (a:A) (b:B): (∃ (bkt: AssocList A B),  (a,b) ∈ bkt.toList ∧ bkt ∈ buckets.1) ↔ ∃ (bkt: AssocList A B),  bkt ∈ (expand size buckets).buckets.1 ∧  (a,b) ∈ bkt.toList := by
+  unfold expand
+  simp
+  simp [HashMap.Imp.expand_go_mem]
+  constructor
+  intro h
+  rcases h with ⟨bkt, ab_mem, bkt_mem⟩
+  use bkt
+  constructor
+  right
+  rw [Array.mem_if_exists] at bkt_mem
+  apply bkt_mem
+  apply ab_mem
+
+
+  intro h
+  rcases h with ⟨bkt, bkt_mem, ab_mem⟩
+  use bkt
+  constructor
+  apply ab_mem
+  cases bkt_mem with
+  | inl h =>
+    unfold Buckets.mk at h
+    simp at h
+    unfold mkArray at h
+    rw [Array.mem_def] at h
+    simp at h
+    rw [List.mem_replicate] at h
+    rcases h with ⟨_, empty⟩
+    rw [empty] at ab_mem
+    unfold AssocList.toList at ab_mem
+    simp at ab_mem
+  | inr h =>
+    rw [Array.mem_if_exists]
+    apply h
+
+
+lemma HashMap.Imp.insert_semantics (m: HashMap.Imp A B) (wf: HashMap.Imp.WF m) (a a': A) (b b':B): (m.insert a b).kv_member a' b' ↔ (m.kv_member a' b' ∧ a ≠ a') ∨ (a, b) = (a', b') :=
+by
+  rw [← Imp.kv_member_iff_in_kv (wf:=wf), ← Imp.kv_member_iff_in_kv (wf:= Imp.WF.insert wf)]
+  cases m with
+  | mk size buckets =>
+    unfold insert
+    simp
+    rw [cond_eq_if]
+    unfold kv
+    unfold Buckets.kv
+    simp
+    rw [Array.foldl_union, Array.foldl_union]
+
+    split
+    simp
+    unfold Buckets.update
+    unfold Array.uset
+    simp only [Array.mem_set]
+    constructor
+    intro h
+    rcases h with ⟨l, h⟩
+    rcases h with ⟨get_l, ab_l⟩
+    cases get_l with
+    | inl replace =>
+      rw [replace] at ab_l
+      rw [← AssocList.mem_containsKeyValue_iff_mem_toList] at ab_l
+      simp at ab_l
+      admit
+    | inr h =>
+      left
+      constructor
+      use l
+      constructor
+
+    admit
+
+    simp
+    split
+    simp
+    unfold Buckets.update
+    unfold Array.uset
+    simp
+    simp [Array.mem_set]
+
+    admit
+
+
+    rw [← HashMap.Imp.expand_preserves_mem]
+
+
+
 
 def HashMap.keys' (m: HashMap A B): Finset A := m.val.keys'
 
@@ -204,7 +612,12 @@ by
   rw [Imp.contains_iff]
   apply m.2
 
+def HashMap.kv_member (m: HashMap A B) (a: A) (b:B): Bool := m.1.kv_member a b
 
+
+lemma HashMap.insert_semantics (m: HashMap A B) (a a': A) (b b':B): (m.insert a b).kv_member a' b' ↔ (m.kv_member a' b' ∧ a' ≠ a) ∨ (a, b) = (a', b') :=
+by
+  sorry
 
 
 end HashMap
